src/Platform/Example64Literal.v
@@ -38,8 +38,6 @@ Goal False.
   (* decoder seems to work :) *)
 Abort.
 
-Definition RiscvMachine := riscv.Platform.RiscvMachine.RiscvMachine Register Empty_set.
-
 (* This example uses the memory only as instruction memory
    TODO make an example which uses memory to store data *)
 Definition zeroedRiscvMachine: RiscvMachine := {|
