src/Platform/MetricRiscvMachine.v
@@ -1,6 +1,8 @@
+Require Import Coq.Strings.String.
 Require Import coqutil.Map.Interface.
 Require Import coqutil.Word.Interface.
 Require Import coqutil.Word.LittleEndian.
+Require Import riscv.Spec.Decode.
 Require Import riscv.Platform.Memory.
 Require Import riscv.Utility.Utility.
 Require Import riscv.Platform.RiscvMachine.
@@ -8,16 +10,12 @@ Require Import riscv.Platform.MetricLogging.
 
 Section Machine.
 
-  Context {Reg: Type}.
   Context {W: Words}.
-  Context {Registers: map.map Reg word}.
+  Context {Registers: map.map Register word}.
   Context {Mem: map.map word byte}.
-  Context {Action: Type}.
-
-  Local Notation RiscvMachineL := (RiscvMachine Reg Action).
 
   Record MetricRiscvMachine := mkMetricRiscvMachine {
-    getMachine :> RiscvMachineL;
+    getMachine :> RiscvMachine;
     getMetrics: MetricLog;
   }.
 
@@ -28,10 +26,10 @@ Section Machine.
   Definition updateMetrics(fm: MetricLog -> MetricLog)(m: MetricRiscvMachine) :=
     withMetrics (fm m.(getMetrics)) m.
 
-  Definition liftGet{A: Type}(getF: RiscvMachineL -> A): (MetricRiscvMachine -> A) :=
+  Definition liftGet{A: Type}(getF: RiscvMachine -> A): (MetricRiscvMachine -> A) :=
     fun m => getF m.
 
-  Definition liftWith{A: Type}(withF: A -> RiscvMachineL -> RiscvMachineL) :=
+  Definition liftWith{A: Type}(withF: A -> RiscvMachine -> RiscvMachine) :=
     fun a m =>
       mkMetricRiscvMachine (withF a m.(getMachine)) m.(getMetrics).
 
@@ -43,8 +41,8 @@ Section Machine.
   Definition withLogItem := liftWith withLogItem.
   Definition withLogItems := liftWith withLogItems.
 
-  Definition forgetMetrics(m: MetricRiscvMachine): RiscvMachineL := m.(getMachine).
-  Definition addMetrics(m: RiscvMachineL)(mc: MetricLog): MetricRiscvMachine :=
+  Definition forgetMetrics(m: MetricRiscvMachine): RiscvMachine := m.(getMachine).
+  Definition addMetrics(m: RiscvMachine)(mc: MetricLog): MetricRiscvMachine :=
     mkMetricRiscvMachine m mc.
 
   Definition putProgram(prog: list MachineInt)(addr: word)(ma: MetricRiscvMachine): MetricRiscvMachine :=
@@ -54,11 +52,9 @@ Section Machine.
 
 End Machine.
 
-Arguments MetricRiscvMachine Reg {W} {Registers} {Mem} Action.
-
 Ltac destruct_RiscvMachine m :=
   lazymatch type of m with
-  | MetricRiscvMachine _ _ =>
+  | MetricRiscvMachine =>
     let r := fresh m "_regs" in
     let p := fresh m "_pc" in
     let n := fresh m "_npc" in
