src/Platform/MinimalLogging.v
@@ -1,4 +1,5 @@
 Require Import Coq.ZArith.BinInt.
+Require Import Coq.Strings.String.
 Require Import riscv.Utility.Monads. Import OStateOperations.
 Require Import riscv.Utility.MonadNotations.
 Require Import riscv.Spec.Decode.
@@ -17,64 +18,52 @@ Section Riscv.
   Context {Mem: map.map word byte}.
   Context {Registers: map.map Register word}.
 
-  Inductive LogEvent :=
-  | EvLoadWord(addr: Z)(i: Instruction)
-  | EvStoreWord(addr: Z)(v: w32).
+  Local Notation empty_mem := (map.empty: Mem).
 
-  Definition mkLogItem(e: LogEvent): LogItem LogEvent :=
-    (* we don't log the memory because that would be too big to read *)
-    ((map.empty, e, nil), (map.empty, nil)).
+  Definition mkLogItemLoad(addr: word)(value: w32): LogItem :=
+    ((empty_mem, "loadWord"%string, [addr]), (empty_mem, [int32ToReg value])).
 
-  Local Notation RiscvMachine := (riscv.Platform.RiscvMachine.RiscvMachine Register Empty_set).
-  Local Notation RiscvMachineL := (riscv.Platform.RiscvMachine.RiscvMachine Register LogEvent).
+  Definition mkLogItemStore(addr: word)(value: w32): LogItem :=
+    ((empty_mem, "storeWord"%string, [addr; int32ToReg value]), (empty_mem, [])).
 
-  Definition downgrade: RiscvMachineL -> RiscvMachine :=
-    fun '(mkRiscvMachine regs pc nextPC mem log) => mkRiscvMachine regs pc nextPC mem nil.
-
-  Definition upgrade: RiscvMachine -> list (LogItem LogEvent) -> RiscvMachineL :=
-    fun '(mkRiscvMachine regs pc nextPC mem _) log => mkRiscvMachine regs pc nextPC mem log.
-
-  Definition liftL0{B: Type}(f: OState RiscvMachine B):  OState RiscvMachineL B :=
-    fun s => let (ob, s') := f (downgrade s) in (ob, upgrade s' s.(getLog)).
-
-  Definition liftL1{A B: Type}(f: A -> OState RiscvMachine B): A -> OState RiscvMachineL B :=
-    fun a s => let (ob, s') := f a (downgrade s) in (ob, upgrade s' s.(getLog)).
-
-  Definition liftL2{A1 A2 B: Type}(f: A1 -> A2 -> OState RiscvMachine B):
-    A1 -> A2 -> OState RiscvMachineL B :=
-    fun a1 a2 s => let (ob, s') := f a1 a2 (downgrade s) in (ob, upgrade s' s.(getLog)).
-
-  Definition liftL3{A1 A2 A3 B: Type}(f: A1 -> A2 -> A3 -> OState RiscvMachine B):
-    A1 -> A2 -> A3 -> OState RiscvMachineL B :=
-    fun a1 a2 a3 s => let (ob, s') := f a1 a2 a3 (downgrade s) in (ob, upgrade s' s.(getLog)).
-
-  Instance IsRiscvMachineL: RiscvProgram (OState RiscvMachineL) word := {
-      getRegister := liftL1 getRegister;
-      setRegister := liftL2 setRegister;
-      getPC := liftL0 getPC;
-      setPC := liftL1 setPC;
-      loadByte   := liftL2 loadByte;
-      loadHalf   := liftL2 loadHalf;
+  Instance IsRiscvMachineL: RiscvProgram (OState RiscvMachine) word := {
+      getRegister := getRegister;
+      setRegister := setRegister;
+      getPC := getPC;
+      setPC := setPC;
+      loadByte   := loadByte;
+      loadHalf   := loadHalf;
       loadWord kind a :=
+        Bind get
+             (fun m =>
+                Bind (Monad := (OState_Monad _)) (* why does Coq infer OStateND_Monad?? *)
+                     (loadWord kind a)
+                     (fun res =>
+                        Bind (Monad := (OState_Monad _)) (* why does Coq infer OStateND_Monad?? *)
+                             (put (withLogItem (mkLogItemLoad a res) m))
+                             (fun _ => Return res)));
+(*
         m <- get;
-        res <- (liftL2 loadWord kind a);
-        put (withLogItem (mkLogItem (EvLoadWord (regToZ_unsigned a) (decode RV64IM (LittleEndian.combine 4 res)))) m);;
+        res <- (loadWord kind a);
+        put (withLogItem (mkLogItemLoad a res));;
         Return res;
-      loadDouble := liftL2 loadDouble;
-      storeByte   := liftL3 storeByte;
-      storeHalf   := liftL3 storeHalf;
+*)
+
+      loadDouble := loadDouble;
+      storeByte   := storeByte;
+      storeHalf   := storeHalf;
 
       storeWord kind a v :=
         Bind get
              (fun m =>
                 Bind (Monad := (OState_Monad _)) (* why does Coq infer OStateND_Monad?? *)
-                     (put (withLogItem (mkLogItem (EvStoreWord (regToZ_unsigned a) v)) m))
+                     (put (withLogItem (mkLogItemStore a v) m))
                      (fun (_: unit) =>
-                        liftL3 storeWord kind a v));
+                        storeWord kind a v));
 
-      storeDouble := liftL3 storeDouble;
-      step := liftL0 step;
-      raiseExceptionWithInfo{A} := liftL3 (raiseExceptionWithInfo (A := A));
+      storeDouble := storeDouble;
+      step := step;
+      raiseExceptionWithInfo{A} := (raiseExceptionWithInfo (A := A));
   }.
 
 End Riscv.
