src/Utility/MMIOTrace.v
@@ -1,15 +1,8 @@
-(*
-We do not do this:
+Require Import Coq.Strings.String.
 
-Inductive MMIOAction := MMInput | MMOutput.
+Definition MMIOAction: Type := string.
+Definition MMInput: MMIOAction := "MMInput"%string.
+Definition MMOutput: MMIOAction := "MMOutput"%string.
 
-Because other libraries (such as bedrock2/bedrock2) don't depend on riscv-coq, but should
-still be able to use the same data type in their trace.
-*)
-
-Definition MMIOAction: Type := bool.
-Definition MMInput: MMIOAction := false.
-Definition MMOutput: MMIOAction := true.
-
-Definition isMMInput(a: MMIOAction): bool := negb a.
-Definition isMMOutput(a: MMIOAction): bool := a.
+Definition isMMInput: MMIOAction -> bool := String.eqb MMInput.
+Definition isMMOutput: MMIOAction -> bool := String.eqb MMOutput.
